Foundation/Modal/Geachean.lean
@@ -1,0 +1,59 @@
+import Foundation.Vorspiel.RelItr
+import Foundation.Vorspiel.BinaryRelations
+
+structure Geachean.Taple where
+  i : ℕ
+  j : ℕ
+  m : ℕ
+  n : ℕ
+
+def Geachean (t : Geachean.Taple) (R : Rel α α) := ∀ {x y z : α}, (R.iterate t.i x y) ∧ (R.iterate t.j x z) → ∃ u, (R.iterate t.m y u) ∧ (R.iterate t.n z u)
+
+
+namespace Geachean
+
+variable {rel : Rel α α}
+
+lemma serial_def : Serial rel ↔ (Geachean ⟨0, 0, 1, 1⟩ rel) := by simp [Geachean, Serial];
+
+lemma reflexive_def : Reflexive rel ↔ (Geachean ⟨0, 0, 1, 0⟩ rel) := by simp [Geachean, Reflexive];
+
+lemma symmetric_def : Symmetric rel ↔ (Geachean ⟨0, 1, 0, 1⟩ rel) := by
+  simp [Geachean, Symmetric];
+  constructor;
+  . rintro h x y z rfl Rxz; exact h Rxz;
+  . intro h x y Rxy; exact h rfl Rxy;
+
+lemma transitive_def : Transitive rel ↔ (Geachean ⟨0, 2, 1, 0⟩ rel) := by
+  simp [Geachean, Transitive];
+  constructor;
+  . rintro h x y z rfl w Rxw Rwz; exact h Rxw Rwz;
+  . intro h x y z Rxy Ryz; exact h rfl y Rxy Ryz
+
+lemma euclidean_def : Euclidean rel ↔ (Geachean ⟨1, 1, 0, 1⟩ rel) := by simp [Geachean, Euclidean];
+
+lemma confluent_def : Confluent rel ↔ (Geachean ⟨1, 1, 1, 1⟩ rel) := by simp [Geachean, Confluent];
+
+lemma extensive_def : Coreflexive rel ↔ (Geachean ⟨0, 1, 0, 0⟩ rel) := by
+  simp [Geachean, Coreflexive];
+  constructor;
+  . rintro h x y z rfl Rxz; have := h Rxz; tauto;
+  . intro h x y Rxy; have := h rfl Rxy; tauto;
+
+lemma functional_def : Functional rel ↔ (Geachean ⟨1, 1, 0, 0⟩ rel) := by
+  simp [Geachean, Functional];
+  constructor <;> tauto;
+
+lemma dense_def : Dense rel ↔ (Geachean ⟨0, 1, 2, 0⟩ rel) := by
+  simp [Geachean, Dense];
+  constructor;
+  . rintro h x y z rfl Rxz; exact h Rxz;
+  . intro h x y Rxy; exact h rfl Rxy;
+
+@[simp]
+lemma satisfies_eq : Geachean (α := α) t (· = ·) := by simp [Geachean];
+
+end Geachean
+
+
+def MultiGeachean (G : Set Geachean.Taple) (R : Rel α α) := ∀ g ∈ G, Geachean g R
