Foundation/Modal/Kripke2/Geach.lean
@@ -1,0 +1,148 @@
+import Foundation.Modal.Hilbert2.Geach
+import Foundation.Modal.Kripke2.Completeness
+import Foundation.Modal.Kripke2.Soundness
+
+namespace LO.Modal
+
+open Formula.Kripke
+
+namespace Kripke
+
+abbrev MultiGeacheanConfluentFrameClass (G : Set Geachean.Taple) : FrameClass := { F | (MultiGeachean G) F.Rel }
+
+instance : (MultiGeacheanConfluentFrameClass G).IsNonempty := by
+  use ⟨Unit, λ _ _ => True⟩;
+  intros t ht x y z h;
+  use x;
+  constructor <;> { apply Rel.iterate.true_any; tauto; }
+
+instance MultiGeacheanFrameClass.isDefinedByGeachAxioms (G) : (MultiGeacheanConfluentFrameClass G).DefinedBy (G.image (λ t => Axioms.Geach t (.atom 0))) := by
+  unfold MultiGeacheanConfluentFrameClass MultiGeachean Axioms.Geach;
+  constructor;
+  intro F;
+  constructor;
+  . rintro hF φ ⟨g, ⟨hg, rfl⟩⟩ V x h;
+    obtain ⟨y, Rxy, hbp⟩ := Satisfies.multidia_def.mp h;
+    apply Satisfies.multibox_def.mpr;
+    intro z Rxz;
+    apply Satisfies.multidia_def.mpr;
+    obtain ⟨u, Ryu, Rzu⟩ := hF g hg ⟨Rxy, Rxz⟩;
+    use u;
+    constructor;
+    . assumption;
+    . exact (Satisfies.multibox_def.mp hbp) Ryu;
+  . rintro h g hg x y z ⟨Rxy, Rxz⟩;
+    let V : Kripke.Valuation F := λ v _ => y ≺^[g.m] v;
+    have : Satisfies ⟨F, V⟩ x (◇^[g.i](□^[g.m](.atom 0))) := by
+      apply Satisfies.multidia_def.mpr;
+      use y;
+      constructor;
+      . assumption;
+      . apply Satisfies.multibox_def.mpr;
+        aesop;
+    have : Satisfies ⟨F, V⟩ x (□^[g.j](◇^[g.n]Formula.atom 0)) := h (Axioms.Geach g (.atom 0)) (by tauto) V x this;
+    have : Satisfies ⟨F, V⟩ z (◇^[g.n]Formula.atom 0) := Satisfies.multibox_def.mp this Rxz;
+    obtain ⟨u, Rzu, Ryu⟩ := Satisfies.multidia_def.mp this;
+    exact ⟨u, Ryu, Rzu⟩;
+
+instance MultiGeacheanFrameClass.isDefinedByGeachHilbertAxioms (ts)
+  : (MultiGeacheanConfluentFrameClass ts).DefinedBy (Hilbert.Geach ts).axioms :=
+  FrameClass.definedBy_with_axiomK (MultiGeacheanFrameClass.isDefinedByGeachAxioms ts)
+
+
+section
+
+variable {F : Frame}
+
+lemma reflexive_of_validate_AxiomT (h : F ⊧ (Axioms.T (.atom 0))) : Reflexive F.Rel := by
+  have : ValidOnFrame F (Axioms.T (.atom 0)) → Reflexive F.Rel := by
+    simpa [Axioms.Geach, MultiGeachean, ←Geachean.reflexive_def] using
+    MultiGeacheanFrameClass.isDefinedByGeachAxioms {⟨0, 0, 1, 0⟩} |>.defines F |>.mpr;
+  exact this h;
+
+lemma transitive_of_validate_AxiomFour (h : F ⊧ (Axioms.Four (.atom 0))) : Transitive F.Rel := by
+  have : ValidOnFrame F (Axioms.Four (.atom 0)) → Transitive F.Rel := by
+    simpa [Axioms.Geach, MultiGeachean, ←Geachean.transitive_def] using
+    MultiGeacheanFrameClass.isDefinedByGeachAxioms {⟨0, 2, 1, 0⟩} |>.defines F |>.mpr;
+  exact this h;
+
+end
+
+end Kripke
+
+
+
+namespace Kripke
+
+variable {S} [System (Formula ℕ) S]
+variable {𝓢 : S} [System.Consistent 𝓢] [System.K 𝓢]
+
+open System
+open FormulaSet
+open canonicalFrame
+open MaximalConsistentSet
+
+lemma canonicalFrame.multigeachean_of_provable_geach
+  (hG : ∀ g ∈ G, ∀ φ, 𝓢 ⊢! ◇^[g.i](□^[g.m]φ) ➝ □^[g.j](◇^[g.n]φ))
+  : MultiGeachean G (canonicalFrame 𝓢).Rel := by
+  intro t ht;
+  rintro X Y Z ⟨RXY, RXZ⟩;
+  have ⟨U, hU⟩ := lindenbaum (𝓢 := 𝓢) (T := □''⁻¹^[t.m]Y.1 ∪ □''⁻¹^[t.n]Z.1) $ by
+    apply intro_union_consistent;
+    rintro Γ Δ ⟨hΓ, hΔ⟩ hC;
+
+    replace hΓ : ∀ φ ∈ Γ, □^[t.m]φ ∈ Y := by simpa using hΓ;
+    have hΓconj : □^[t.m]⋀Γ ∈ Y := iff_mem_multibox_conj.mpr hΓ;
+
+    replace hΔ : ∀ φ ∈ Δ, □^[t.n]φ ∈ Z := by simpa using hΔ;
+    have hZ₁ : □^[t.n]⋀Δ ∈ Z := iff_mem_multibox_conj.mpr hΔ;
+
+    have : □^[t.j](◇^[t.n]⋀Γ) ∈ X := MaximalConsistentSet.mdp
+      (membership_iff.mpr $ Context.of! (hG t ht _))
+      (multirel_def_multidia.mp RXY hΓconj)
+    have hZ₂ : ◇^[t.n]⋀Γ ∈ Z := multirel_def_multibox.mp RXZ this;
+
+    have : 𝓢 ⊢! □^[t.n]⋀Δ ⋏ ◇^[t.n]⋀Γ ➝ ⊥ := by {
+      apply and_imply_iff_imply_imply'!.mpr;
+      exact imp_trans''!
+        (show _ ⊢! □^[t.n]⋀Δ ➝ □^[t.n](∼⋀Γ) by exact imply_multibox_distribute'! $ contra₁'! $ imp_trans''! (and_imply_iff_imply_imply'!.mp hC) (and₂'! neg_equiv!))
+        (show _ ⊢! □^[t.n](∼⋀Γ) ➝ (◇^[t.n]⋀Γ) ➝ ⊥ by exact imp_trans''! (contra₁'! $ and₁'! $ multidia_duality!) (and₁'! neg_equiv!));
+    }
+    have : 𝓢 ⊬ □^[t.n]⋀Δ ⋏ ◇^[t.n]⋀Γ ➝ ⊥ := (def_consistent.mp (Z.consistent)) (Γ := [□^[t.n]⋀Δ, ◇^[t.n]⋀Γ]) $ by
+      suffices □^[t.n]⋀Δ ∈ ↑Z ∧ ◇^[t.n]⋀Γ ∈ ↑Z by simpa;
+      constructor <;> assumption;
+    contradiction;
+  use U;
+  simp only [Set.union_subset_iff] at hU;
+  constructor;
+  . apply multirel_def_multibox.mpr; apply hU.1;
+  . apply multirel_def_multibox.mpr; apply hU.2;
+
+end Kripke
+
+
+namespace Hilbert.Geach
+
+open Kripke
+
+instance Kripke.Consistent : System.Consistent (Hilbert.Geach G) := Kripke.Hilbert.instConsistent (Kripke.MultiGeacheanConfluentFrameClass G)
+
+instance Kripke.Canonical : Canonical (Hilbert.Geach G) (MultiGeacheanConfluentFrameClass G) := ⟨by
+  apply canonicalFrame.multigeachean_of_provable_geach;
+  intro t ht φ;
+  apply Hilbert.Deduction.maxm!;
+  unfold Hilbert.axiomInstances;
+  use Axioms.Geach t (.atom 0);
+  constructor;
+  . simp only [Hilbert.axioms];
+    right;
+    aesop;
+  . use (λ _ => φ); simp;
+⟩
+
+instance Kripke.Complete : Complete (Hilbert.Geach G) (MultiGeacheanConfluentFrameClass G) := inferInstance
+
+end Hilbert.Geach
+
+
+end LO.Modal
