Foundation/Modal/Kripke2/K.lean
@@ -1,0 +1,15 @@
+import Foundation.Modal.Hilbert2.K
+import Foundation.Modal.Kripke2.Soundness
+import Foundation.Modal.Kripke2.Completeness
+
+namespace LO.Modal
+
+namespace Hilbert.K
+
+instance : System.Consistent (Hilbert.K) := Kripke.Hilbert.instConsistent Kripke.AllFrameClass
+
+instance : Complete (Hilbert.K) (Kripke.AllFrameClass) := Kripke.instCompleteOfCanonical trivial
+
+end Hilbert.K
+
+end LO.Modal
