Foundation/Modal/Kripke2/S4.lean
@@ -1,0 +1,24 @@
+import Foundation.Modal.Kripke2.Geach
+
+namespace LO.Modal
+
+open Kripke
+open Geachean
+
+abbrev Kripke.ReflexiveTransitiveFrameClass : FrameClass := { F | Reflexive F ∧ Transitive F }
+
+namespace Hilbert.S4
+
+instance Kripke.Consistent : System.Consistent (Hilbert.S4) := by
+  convert Hilbert.Geach.Kripke.Consistent (G := {⟨0, 0, 1, 0⟩, ⟨0, 2, 1, 0⟩});
+  exact eq_Geach;
+
+instance Kripke.Complete : Complete (Hilbert.S4) (Kripke.ReflexiveTransitiveFrameClass) := by
+  convert Hilbert.Geach.Kripke.Complete (G := {⟨0, 0, 1, 0⟩, ⟨0, 2, 1, 0⟩});
+  . exact eq_Geach;
+  . unfold ReflexiveTransitiveFrameClass MultiGeacheanConfluentFrameClass MultiGeachean;
+    simp [Geachean.reflexive_def, Geachean.transitive_def];
+
+end Hilbert.S4
+
+end LO.Modal
